Setlec/SetR.lean
@@ -34,6 +34,7 @@ import Setlec.SetR.Install.IndMemberS
 import Setlec.SetR.Install.IndMembersS
 import Setlec.SetR.Install.SwapS
 import Setlec.SetR.Install.IotaRuleS
+import Setlec.SetR.Install.IndRecsS
 import Setlec.SetR.Examples
 import Setlec.SetR.Bridge.Env
 import Setlec.SetR.Bridge.Claims
